

(a) poisson $p(x(t)=k) = \frac{e^{-\lambda t} (\lambda t)^k}{k!}$ $\lambda = 1$

$$L_1 = \{0, 1, 2\} \quad p(x=k) = \frac{e^{-\lambda} \lambda^k}{k!}$$

$$p_{01} = e^{-1} \quad p_{02} = e^{-1} \quad p_{00} = 1 - e^{-1} - e^{-1} = 1 - 2e^{-1}$$

$$p_{10} = 1 - e^{-1} \quad p_{11} = e^{-1} \quad p_{12} = 0$$

$$p_{20} = 1 - 2e^{-1} \quad p_{21} = e^{-1} \quad p_{22} = e^{-1}$$

$$p = \begin{bmatrix} 1-2e^{-1} & e^{-1} & e^{-1} \\ 1-e^{-1} & e^{-1} & 0 \\ 1-2e^{-1} & e^{-1} & e^{-1} \end{bmatrix}$$

Sojourn time $T_{00} = \frac{1}{1-p_{00}} = \frac{1}{2e^{-1}} = 0.5e$

$$T_{11} = \frac{1}{1-p_{11}} = \frac{1}{1-e^{-1}}$$

$$T_{22} = \frac{1}{1-p_{22}} = \frac{1}{1-e^{-1}}$$

(b)

$$Yp = Y \quad \Sigma Y = 1$$

$$[Y_1 \ Y_2 \ Y_3] \begin{bmatrix} 1-2e^{-1} & e^{-1} & e^{-1} \\ 1-e^{-1} & e^{-1} & 0 \\ 1-2e^{-1} & e^{-1} & e^{-1} \end{bmatrix} = [Y_1 \ Y_2 \ Y_3]$$

$$\begin{cases} (1-2e^{-1})Y_1 + (1-e^{-1})Y_2 + (1-2e^{-1})Y_3 = Y_1 \\ (Y_1 + Y_2 + Y_3)e^{-1} = Y_2 \\ (Y_1 + Y_3)e^{-1} = Y_3 \\ Y_1 + Y_2 + Y_3 = 1 \end{cases}$$

$$Y_3 + Y_2 e^{-1} = Y_2 \Rightarrow Y_3 = (1-e^{-1})Y_2$$

$$(Y_1 + (1-e^{-1})Y_2)e^{-1} = (1-e^{-1})Y_2$$

$$Y_1 e^{-1} + e^{-1}(1-e^{-1})Y_2 = (1-e^{-1})Y_2$$

$$Y_1 = e(1-e^{-1})^2 Y_2$$

$$e(1-e^{-1})^2 Y_2 + Y_2 + (1-e^{-1})Y_2 = 1 \Rightarrow Y_2 = 0.368$$

$$Y_1 = 0.400$$

$$Y_3 = 0.233$$

(C)

$$L_k = \{0, 1, 2, 3, \dots, m\}$$

$$\frac{e^{-\lambda} \lambda^k}{k!}$$

$$P_{00} = P(N \neq M) = 1 - P_{01} - P_{02} - P_{03} - \dots - P_{0(m-1)} - P_{0m}$$

$$= 1 - \frac{e^{-1}}{(m-1)!} - \frac{e^{-1}}{(m-2)!} - \frac{e^{-1}}{(m-3)!} - \dots - \frac{e^{-1}}{1!} - \frac{e^{-1}}{0!}$$

$$= 1 - \sum_{n=0}^{m-1} \frac{e^{-1}}{n!}$$

$$P_{11} = \frac{e^{-1}}{0!} = e^{-1} \Rightarrow P_{ii} = e^{-1}$$